update CH12.

Coq/Coq19.v
@@ -9,9 +9,53 @@ Require Import Coq.Arith.EqNat.
 Require Import Coq.omega.Omega. 
 Require Import Coq.Lists.List. 
 Require Import Unicode.Utf8.
+Require Export Coq.Strings.String. 
+Require Import Setoid.
 Import ListNotations.
 
-Inductive aexp : Type :=   
+Definition beq_string x y :=   if string_dec x y then true else false. 
+
+Theorem beq_string_refl : ∀ s, true = beq_string s s. 
+Proof. 
+  intros s. unfold beq_string. destruct (string_dec s s) as [|Hs]. 
+  - reflexivity.   
+  - destruct Hs. reflexivity. 
+Qed.
+
+Theorem beq_string_true_iff : ∀ x y : string,   beq_string x y = true ↔ x = y. 
+Proof. 
+  intros x y. 
+  unfold beq_string. 
+  destruct (string_dec x y) as [|Hs]. 
+  - subst. split. auto. auto.
+  - split. 
+    + intros contra. inversion contra.
+    + intros H. destruct Hs. auto.
+Qed.
+
+Theorem beq_string_false_iff : ∀ x y : string,   beq_string x y = false   ↔ x ≠ y. 
+Proof. 
+  intros x y. rewrite <- beq_string_true_iff. 
+  rewrite not_true_iff_false. reflexivity. 
+Qed.
+
+Definition total_map (A:Type) := string → A.
+
+Definition t_empty {A:Type} (v : A) : total_map A :=   (fun _ => v).
+
+Definition t_update {A:Type} (m : total_map A) (x : string) (v : A) := 
+  fun x' => if beq_string x x' then v else m x'.
+
+Notation "'_' '!->' v" := (t_empty v)
+  (at level 100, right associativity).
+Notation "x '!->' v ';' m" := (t_update m x v)
+                              (at level 100, v at next level, right associativity).
+
+Definition state := total_map nat. 
+
+Module EXP_TRY.
+
+Inductive aexp : Type :=
   | ANum : nat → aexp   
   | APlus : aexp → aexp → aexp   
   | AMinus : aexp → aexp → aexp   
@@ -156,4 +200,253 @@ Inductive aevalR : aexp → nat → Prop :=
       (e1 \\ n1) → (e2 \\ n2) → (AMult e1 e2) \\ (n1 * n2)
 
   where "e '\\' n" := (aevalR e n) : type_scope.
+
+Theorem aeval_iff_aevalR' : ∀a n,
+  (a \\ n) ↔ aeval a = n.
+Proof.
+  split.
+  - intros H; induction H; subst; reflexivity.
+  - generalize dependent n.
+    induction a; simpl; intros; subst; constructor;
+       try apply IHa1; try apply IHa2; reflexivity.
+Qed.
+
+Inductive bevalR: bexp → bool → Prop :=
+  | E_BTrue :  bevalR BTrue  true
+  | E_BFalse : bevalR BFalse false
+  | E_BEq (a1 a2 : aexp) (n1 n2 : nat) : (a1 \\ n1) -> (a2 \\ n2) -> bevalR (BEq a1 a2) (n1  =? n2)
+  | E_BLe (a1 a2 : aexp) (n1 n2 : nat) : (a1 \\ n1) -> (a2 \\ n2) -> bevalR (BLe a1 a2) (n1 <=? n2)
+  | E_BNot (b : bexp) (m : bool) : bevalR b m -> bevalR (BNot b) (negb m)
+  | E_BAnd (b1 b2 : bexp) (m1 m2 : bool) : bevalR b1 m1 -> bevalR b2 m2 -> bevalR (BAnd b1 b2) (andb m1 m2).
+
+Lemma beval_iff_bevalR : ∀b bv,
+  bevalR b bv ↔ beval b = bv.
+Proof.
+  split.
+  - intros H; induction H; try (subst; auto);
+    try (apply aeval_iff_aevalR' in H;
+         apply aeval_iff_aevalR' in H0;
+         subst; auto).
+  - generalize dependent bv;
+    induction b;
+    try (intros; subst; constructor; apply aeval_iff_aevalR'; auto);
+    try (intros; simpl in H; subst; constructor; try apply IHb; try apply IHb1; try apply IHb2; auto).
+Qed.
+
+End EXP_TRY.
+
+Inductive aexp : Type :=
+  | AId : string → aexp
+  | ANum : nat → aexp   
+  | APlus : aexp → aexp → aexp   
+  | AMinus : aexp → aexp → aexp   
+  | AMult : aexp → aexp → aexp. 
+
+Inductive bexp : Type :=   
+  | BTrue : bexp   
+  | BFalse : bexp   
+  | BEq : aexp → aexp → bexp   
+  | BLe : aexp → aexp → bexp   
+  | BNot : bexp → bexp   
+  | BAnd : bexp → bexp → bexp.
+
+Fixpoint aeval (st : state) (a : aexp) : nat :=
+  match a with
+  | ANum n => n
+  | AId x => st x
+  | APlus a1 a2 => (aeval st a1) + (aeval st a2)
+  | AMinus a1 a2 => (aeval st a1) - (aeval st a2)
+  | AMult a1 a2 => (aeval st a1) * (aeval st a2)
+  end.
+
+Fixpoint beval (st : state) (b : bexp) : bool :=
+  match b with
+  | BTrue => true
+  | BFalse => false
+  | BEq a1 a2 => (aeval st a1) =? (aeval st a2)
+  | BLe a1 a2 => (aeval st a1) <=? (aeval st a2)
+  | BNot b1 => negb (beval st b1)
+  | BAnd b1 b2 => andb (beval st b1) (beval st b2)
+  end.
+
+Definition W : string := "W".
+Definition X : string := "X".
+Definition Y : string := "Y".
+Definition Z : string := "Z".
+
+Coercion AId : string >-> aexp.
+Coercion ANum : nat >-> aexp.
+Definition bool_to_bexp (b : bool) : bexp :=
+  if b then BTrue else BFalse.
+Coercion bool_to_bexp : bool >-> bexp.
+Bind Scope imp_scope with aexp.
+Bind Scope imp_scope with bexp.
+Delimit Scope imp_scope with imp.
+Notation "x + y" := (APlus x y) (at level 50, left associativity) : imp_scope.
+Notation "x - y" := (AMinus x y) (at level 50, left associativity) : imp_scope.
+Notation "x * y" := (AMult x y) (at level 40, left associativity) : imp_scope.
+Notation "x ≤ y" := (BLe x y) (at level 70, no associativity) : imp_scope.
+Notation "x = y" := (BEq x y) (at level 70, no associativity) : imp_scope.
+Notation "x && y" := (BAnd x y) (at level 40, left associativity) : imp_scope.
+Notation "'~' b" := (BNot b) (at level 75, right associativity) : imp_scope.
+Definition example_aexp := (3 + (X * 2))%imp : aexp.
+Definition example_bexp := (true && ~(X ≤ 4))%imp : bexp.
+
+Definition empty_st := (_ !-> 0).
+Notation "a '!->' x" := (t_update empty_st a x) (at level 100).
+
+Example aexp1 :
+    aeval (X !-> 5) (3 + (X * 2))%imp
+  = 13.
+Proof. reflexivity. Qed.
+
+Inductive com : Type :=
+  | CSkip
+  | CAss (x : string) (a : aexp)
+  | CSeq (c1 c2 : com)
+  | CIf (b : bexp) (c1 c2 : com)
+  | CWhile (b : bexp) (c : com).
+
+Bind Scope imp_scope with com.
+Notation "'SKIP'" :=
+   CSkip : imp_scope.
+Notation "x '::=' a" :=
+  (CAss x a) (at level 60) : imp_scope.
+Notation "c1 ;; c2" :=
+  (CSeq c1 c2) (at level 80, right associativity) : imp_scope.
+Notation "'WHILE' b 'DO' c 'END'" :=
+  (CWhile b c) (at level 80, right associativity) : imp_scope.
+Notation "'IFB' c1 'THEN' c2 'ELSE' c3 'FI'" :=
+  (CIf c1 c2 c3) (at level 80, right associativity) : imp_scope.
+
+Open Scope imp_scope.
+Fixpoint ceval_fun_no_while (st : state) (c : com)
+                          : state :=
+  match c with
+    | SKIP =>
+        st
+    | x ::= a1 =>
+        (x !-> (aeval st a1) ; st)
+    | c1 ;; c2 =>
+        let st' := ceval_fun_no_while st c1 in
+        ceval_fun_no_while st' c2
+    | IFB b THEN c1 ELSE c2 FI =>
+        if (beval st b)
+          then ceval_fun_no_while st c1
+          else ceval_fun_no_while st c2
+    | WHILE b DO c END =>
+        st (* bogus *)
+  end.
+Close Scope imp_scope.
+
+Reserved Notation "st '=[' c ']⇒' st'"
+                  (at level 40).
+Inductive ceval : com → state → state → Prop :=
+  | E_Skip : ∀st,
+      st =[ SKIP ]⇒ st
+  | E_Ass : ∀st a1 n x,
+      aeval st a1 = n →
+      st =[ x ::= a1 ]⇒ (x !-> n ; st)
+  | E_Seq : ∀c1 c2 st st' st'',
+      st =[ c1 ]⇒ st' →
+      st' =[ c2 ]⇒ st'' →
+      st =[ c1 ;; c2 ]⇒ st''
+  | E_IfTrue : ∀st st' b c1 c2,
+      beval st b = true →
+      st =[ c1 ]⇒ st' →
+      st =[ IFB b THEN c1 ELSE c2 FI ]⇒ st'
+  | E_IfFalse : ∀st st' b c1 c2,
+      beval st b = false →
+      st =[ c2 ]⇒ st' →
+      st =[ IFB b THEN c1 ELSE c2 FI ]⇒ st'
+  | E_WhileFalse : ∀b st c,
+      beval st b = false →
+      st =[ WHILE b DO c END ]⇒ st
+  | E_WhileTrue : ∀st st' st'' b c,
+      beval st b = true →
+      st =[ c ]⇒ st' →
+      st' =[ WHILE b DO c END ]⇒ st'' →
+      st =[ WHILE b DO c END ]⇒ st''
+
+  where "st =[ c ]⇒ st'" := (ceval c st st').
+
+Example ceval_example1:
+  empty_st =[
+     X ::= 2;;
+     IFB X ≤ 1
+       THEN Y ::= 3
+       ELSE Z ::= 4
+     FI
+  ]⇒ (Z !-> 4 ; X !-> 2).
+Proof.
+  apply E_Seq with (X !-> 2).
+  - apply E_Ass. auto.
+  - apply E_IfFalse.
+    + auto.
+    + apply E_Ass. auto.
+Qed.
+
+Example ceval_example2:
+  empty_st =[
+    X ::= 0;; Y ::= 1;; Z ::= 2
+  ]⇒ (Z !-> 2 ; Y !-> 1 ; X !-> 0).
+Proof.
+  apply E_Seq with (X !-> 0).
+  - apply E_Ass. auto.
+  - apply E_Seq with (Y !-> 1 ; X !-> 0).
+    + apply E_Ass. auto.
+    + apply E_Ass. auto.
+Qed.
+
+Definition pup_to_n : com :=
+  (Y ::= 0 ;;
+  WHILE ~(X = 0) DO
+    Y ::= Y + X ;;
+    X ::= X - 1
+  END)%imp.
+
+Theorem pup_to_2_ceval :
+  (X !-> 2) =[
+    pup_to_n
+  ]⇒ (X !-> 0 ; Y !-> 3 ; X !-> 1 ; Y !-> 2 ; Y !-> 0 ; X !-> 2).
+Proof.
+  unfold pup_to_n.
+  apply E_Seq with (Y !-> 0 ; X !-> 2).
+  - apply E_Ass. auto.
+  - apply E_WhileTrue with (X !-> 1; Y !-> 2; Y !-> 0; X !-> 2).
+    + auto.
+    + apply E_Seq with (Y !-> 2; Y !-> 0; X !-> 2). apply E_Ass. auto.
+      apply E_Ass. auto.
+    + apply E_WhileTrue with (X !-> 0; Y !-> 3; X !-> 1; Y !-> 2; Y !-> 0; X !-> 2).
+      ++ auto.
+      ++ apply E_Seq with (Y !-> 3; X !-> 1; Y !-> 2; Y !-> 0; X !-> 2). apply E_Ass. auto.
+         apply E_Ass. auto.
+      ++ apply E_WhileFalse. auto.
+Qed.
+
+Theorem ceval_deterministic: ∀c st st1 st2,
+     st =[ c ]⇒ st1 →
+     st =[ c ]⇒ st2 →
+     st1 = st2.
+Proof.
+  intros c st st1 st2 E1 E2. generalize dependent st2.
+  induction E1; intros st2 E2; inversion E2; subst.
+  - auto.
+  - auto.
+  - assert (st' = st'0) as EQ1.
+    { apply IHE1_1; assumption. }
+    subst st'0.
+    apply IHE1_2. assumption.
+  - apply IHE1. auto.
+  - rewrite H in H5. inversion H5.
+  - rewrite H in H5. inversion H5.
+  - apply IHE1. auto.
+  - auto.
+  - rewrite H in H2. inversion H2.
+  - rewrite H in H4. inversion H4.
+  - assert (st' = st'0) as EQ1.
+    { apply IHE1_1; assumption. }
+    subst st'0.
+    apply IHE1_2. assumption.
+Qed.
 
